adding macros to formulas

translator/lean/llzk/Llzk/SymEx/FFConstraints.lean
@@ -11,12 +11,12 @@ open Llzk.Language.Core.Syntax.AST
 /- Metadata for FF variables -/
 structure FFVarMetaData where
   orig_name : String
-  cmd_meta_data : CmdMetaData
+  src_info : SrcInfo
   deriving Repr, BEq, Inhabited
 
 structure BoolVarMetaData where
   orig_name : String
-  cmd_meta_data : CmdMetaData
+  src_info : SrcInfo
   deriving Repr, BEq, Inhabited
 
 /- A variable in the finite field constraint system -/
@@ -61,6 +61,8 @@ instance : Ord BoolVar where
     | .eq => compare a.id b.id -- Names equal? Check IDs
     | ord => ord               -- Names different? Return that order
 
+abbrev Var := FFVar ⊕ BoolVar
+
 /- Term is a polynomial expression over finite fields -/
 inductive FFTerm (c : ZKConfig) where
   | const : FF c →  FFTerm c
@@ -72,17 +74,70 @@ inductive FFTerm (c : ZKConfig) where
 
 /- A formula is a boolean formula with P(x)=0 as atoms.  -/
 inductive FFFormula (c : ZKConfig) where
-  | bool   : BoolVar → FFFormula c          -- A boolean variable
+  | true   : FFFormula c
+  | false  : FFFormula c
+  | bool   : BoolVar → FFFormula c        -- A boolean variable
   | eqZero : FFTerm c → FFFormula c       -- P(x) = 0
-  | and    : FFFormula c → FFFormula c → FFFormula c
-  | or     : FFFormula c → FFFormula c → FFFormula c
-  | not    : FFFormula c → FFFormula c
+  | and    : FFFormula c → FFFormula c → FFFormula c -- and
+  | or     : FFFormula c → FFFormula c → FFFormula c -- or
+  | not    : FFFormula c → FFFormula c -- negation
   | ite    : FFFormula c → FFFormula c → FFFormula c → FFFormula c  -- if-then-else
   | imply  : FFFormula c → FFFormula c → FFFormula c  -- implication
   | iff    : FFFormula c → FFFormula c → FFFormula c  -- if and only if
-  | true   : FFFormula c
-  | false  : FFFormula c
+  | call   : String → List Var → FFFormula c  -- macro call
   deriving Repr, BEq, Inhabited
+
+/- Trivial definition for size of formula, to be used for proving termination -/
+def sizeOfFormula {c : ZKConfig} : FFFormula c → Nat
+  | .true | .false => 1
+  | .bool _ => 1
+  | .eqZero _ => 1
+  | .and a b | .or a b | .imply a b | .iff a b => 1 + sizeOfFormula a + sizeOfFormula b
+  | .not a => 1 + sizeOfFormula a
+  | .ite c t e => 1 + sizeOfFormula c + sizeOfFormula t + sizeOfFormula e
+  | .call _ _ => 1
+
+/- A macro is a named formula with parameters -/
+structure FFMacro (c : ZKConfig) where
+  name : String
+  params : List Var
+  body : FFFormula c
+  deriving Repr, BEq, Inhabited
+
+/- A constraint system consists of a list of macros and a main formula -/
+structure FFConstraintSystem (c : ZKConfig) where
+  macros : List (FFMacro c)
+  formula : FFFormula c
+  deriving Repr, BEq, Inhabited
+
+
+/-- Fetch a macro by name from a constraint system. Throws an error if the macro is not found. -/
+def fetchMacro {c : ZKConfig}
+    (ms : List (FFMacro c)) (name : String) : Except String (FFMacro c × List (FFMacro c)) :=
+  match ms with
+  | [] => Except.error s!"Macro {name} not found"
+  | m :: rest =>
+      if m.name == name then Except.ok (m, rest)
+      else fetchMacro rest name
+
+/- fetchMacro returns a smaller list -/
+theorem fetchMacroLT {c : ZKConfig} (ms ms' : List (FFMacro c)) (name : String) (m : FFMacro c) :
+  fetchMacro ms name = Except.ok (m, ms') → ms'.length < ms.length := by
+  cases ms with
+  | nil => simp [fetchMacro]
+  | cons head tail =>
+      simp only [fetchMacro]
+      by_cases h : head.name = name
+      · simp only [h, BEq.rfl, ↓reduceIte, Except.ok.injEq, Prod.mk.injEq, List.length_cons,
+        Order.lt_add_one_iff, and_imp] at *
+        intro h1 h2
+        rw [h2]
+      · simp only [h, not_false_eq_true, beq_iff_eq, ↓reduceIte, List.length_cons,
+        Order.lt_add_one_iff] at *
+        intro h1
+        have h2 := fetchMacroLT tail ms' name m h1
+        grind
+
 
 /- An assignment maps variables to FF values -/
 structure Assignment (c : ZKConfig) where
@@ -90,6 +145,29 @@ structure Assignment (c : ZKConfig) where
   bool : ℕ → Bool
   deriving Inhabited
 
+/- Renaming of variables for macro calls -/
+def newAssignment' {c : ZKConfig}
+   (assign : Assignment c)
+   (orginNames newNames : List Var)
+   (ffMap : ℕ → FF c)
+   (boolMap : ℕ → Bool) : Except String (Assignment c) :=
+  match orginNames, newNames with
+  | [], [] => Except.ok { ff := ffMap, bool := boolMap }
+  | (.inl org) :: orgs, (.inl new) :: news =>
+    let ffMap' : ℕ → FF c := fun id => if id == new.id then assign.ff org.id else ffMap id
+    newAssignment' assign orgs news ffMap' boolMap
+  | (.inr org) :: orgs, (.inr new) :: news =>
+    let boolMap' : ℕ → Bool := fun id => if id == new.id then assign.bool org.id else boolMap id
+    newAssignment' assign orgs news ffMap boolMap'
+  -- This case should not happen if the input lists are well-formed. Later will throw an exception.
+  | _, _ => Except.error "Mismatched variable lists"
+
+def newAssignment {c : ZKConfig}
+   (assign : Assignment c)
+   (orginNames newNames : List Var) : Except String (Assignment c) :=
+  let ffMap : ℕ → FF c := fun _id => 0
+  let boolMap : ℕ → Bool := fun _id => false
+  newAssignment' assign orginNames newNames ffMap boolMap
 
 /- Evaluate Terms to FF values -/
 def eval_term {c : ZKConfig} (assign : Assignment c) (t : FFTerm c) : FF c :=
@@ -101,23 +179,50 @@ def eval_term {c : ZKConfig} (assign : Assignment c) (t : FFTerm c) : FF c :=
   | .mul a b => (eval_term assign a) * (eval_term assign b)
 
 /- Evaluate Formulas to Propositions (Prop) -/
-def eval_formula {c : ZKConfig} (assign : Assignment c) (f : FFFormula c) : Bool :=
+def eval_formula {c : ZKConfig}
+   (assign : Assignment c) (f : FFFormula c) (ms : List (FFMacro c)) : Except String Bool := do
   match f with
-  | .bool v   => assign.bool v.id
-  | .eqZero t => eval_term assign t = 0
-  | .and a b  => (eval_formula assign a) && (eval_formula assign b)
-  | .or a b   => (eval_formula assign a) || (eval_formula assign b)
-  | .not a    => !(eval_formula assign a)
-  | .ite c t e => if eval_formula assign c then eval_formula assign t else eval_formula assign e
-  | .imply a b => !(eval_formula assign a) || (eval_formula assign b)
-  | .iff a b   => (eval_formula assign a) == (eval_formula assign b)
-  | .true     => true
-  | .false    => false
+  | .true     => return true
+  | .false    => return false
+  | .bool v   => return assign.bool v.id
+  | .eqZero t => return eval_term assign t = 0
+  | .and a b  => return (← eval_formula assign a ms) && (← eval_formula assign b ms)
+  | .or a b   => return (← eval_formula assign a ms) || (← eval_formula assign b ms)
+  | .not a    => return !(← eval_formula assign a ms)
+  | .ite c t e => if (← eval_formula assign c ms) then eval_formula assign t ms
+                  else eval_formula assign e ms
+  | .imply a b => return !(← eval_formula assign a ms) || (← eval_formula assign b ms)
+  | .iff a b   => return (← eval_formula assign a ms) == (← eval_formula assign b ms)
+  | .call name args =>
+     match _h_fetchm: fetchMacro ms name with
+     | Except.error e => Except.error e
+     | Except.ok (m,ms') =>
+       let newAssign ← newAssignment assign args m.params
+       eval_formula newAssign m.body ms'
+termination_by (ms.length, sizeOfFormula f)
+decreasing_by
+  any_goals
+    apply Prod.Lex.right
+    simp only [sizeOfFormula]
+    grind
+  -- the call to a macro
+  apply Prod.Lex.left
+  apply fetchMacroLT ms ms' name m _h_fetchm
 
-/- Satisfiability: does there EXIST an assignment σ such that evalFormula is true? -/
-def is_sat {c : ZKConfig} (f : FFFormula c) : Prop :=
-  ∃ (σ : Assignment c), eval_formula σ f = true
+/- Satisfiability of a formula:
 
+   Does there EXIST an assignment σ such that evalFormula is true?
+-/
+def is_sat_formula {c : ZKConfig} (f : FFFormula c) (ms : List (FFMacro c)) : Prop :=
+  ∃ (σ : Assignment c), eval_formula σ f ms = Except.ok true
+
+
+/- Satisfiability of a system:
+
+   Does there EXIST an assignment σ such that the main formula is true?
+-/
+def is_sat_sys {c : ZKConfig} (sys : FFConstraintSystem c) : Prop :=
+  is_sat_formula sys.formula sys.macros
 
 
 /- The next functions are used to collect all variables that are used in a formula.
@@ -132,51 +237,57 @@ abbrev BoolVarSet := Std.TreeSet BoolVar compare
 abbrev emptyBoolVarSet : BoolVarSet := Std.TreeSet.empty
 
 /- Collect variables from a Term into the accumulator set -/
-partial def collect_vars_term {c : ZKConfig} (acc : FFVarSet) (t : FFTerm c) : FFVarSet :=
+partial def collectVarsTerm {c : ZKConfig} (acc : FFVarSet) (t : FFTerm c) : FFVarSet :=
   match t with
   | .const _   => acc
   | .var v     => acc.insert v
   | .add a b   =>
-      let acc' := collect_vars_term acc a
-      collect_vars_term acc' b
+      let acc' := collectVarsTerm acc a
+      collectVarsTerm acc' b
   | .sub a b   =>
-      let acc' := collect_vars_term acc a
-      collect_vars_term acc' b
+      let acc' := collectVarsTerm acc a
+      collectVarsTerm acc' b
   | .mul a b   =>
-      let acc' := collect_vars_term acc a
-      collect_vars_term acc' b
+      let acc' := collectVarsTerm acc a
+      collectVarsTerm acc' b
 
 /- Collect variables from a Formula into the accumulator set -/
-partial def collect_vars_formula {c : ZKConfig}
+partial def collectVarsFormula {c : ZKConfig}
   (acc : FFVarSet × BoolVarSet) (f : FFFormula c) : FFVarSet × BoolVarSet :=
   match f with
-  | .eqZero t => (collect_vars_term acc.1 t, acc.2)
-  | .bool v   => (acc.1, acc.2.insert v)
-  | .and a b  =>
-      let acc' := collect_vars_formula acc a
-      collect_vars_formula acc' b
-  | .or a b   =>
-      let acc' := collect_vars_formula acc a
-      collect_vars_formula acc' b
-  | .not a    => collect_vars_formula acc a
-  | .ite c t e =>
-      let acc' := collect_vars_formula acc c
-      let acc'' := collect_vars_formula acc' t
-      collect_vars_formula acc'' e
-  | .imply a b =>
-      let acc' := collect_vars_formula acc a
-      collect_vars_formula acc' b
-  | .iff a b   =>
-      let acc' := collect_vars_formula acc a
-      collect_vars_formula acc' b
   | .true     => acc
   | .false    => acc
+  | .eqZero t => (collectVarsTerm acc.1 t, acc.2)
+  | .bool v   => (acc.1, acc.2.insert v)
+  | .and a b  =>
+      let acc' := collectVarsFormula acc a
+      collectVarsFormula acc' b
+  | .or a b   =>
+      let acc' := collectVarsFormula acc a
+      collectVarsFormula acc' b
+  | .not a    => collectVarsFormula acc a
+  | .ite c t e =>
+      let acc' := collectVarsFormula acc c
+      let acc'' := collectVarsFormula acc' t
+      collectVarsFormula acc'' e
+  | .imply a b =>
+      let acc' := collectVarsFormula acc a
+      collectVarsFormula acc' b
+  | .iff a b   =>
+      let acc' := collectVarsFormula acc a
+      collectVarsFormula acc' b
+  | .call _ args =>
+      args.foldl (fun acc var =>
+        match var with
+        | .inl ffVar => (acc.1.insert ffVar, acc.2)
+        | .inr boolVar => (acc.1, acc.2.insert boolVar)
+      ) acc
 
 /- Returns a list of all unique variables in the formula -/
-def collect_vars {c : ZKConfig} (f : FFFormula c) : List FFVar × List BoolVar :=
+def collectVars {c : ZKConfig} (f : FFFormula c) : List FFVar × List BoolVar :=
   let emptyFFSet : FFVarSet := emptyFFVarSet
   let emptyBoolSet : BoolVarSet := emptyBoolVarSet
-  let finalSet := collect_vars_formula (emptyFFSet, emptyBoolSet) f
+  let finalSet := collectVarsFormula (emptyFFSet, emptyBoolSet) f
   -- Convert the set back to a List for your SMT printer
   (finalSet.1.toList, finalSet.2.toList)
 
@@ -187,124 +298,153 @@ def collect_vars {c : ZKConfig} (f : FFFormula c) : List FFVar × List BoolVar :
 -/
 
 /- Generates spaces for indentation -/
-def get_indent (level : Nat) : String :=
+def getIndent (level : Nat) : String :=
   String.ofList (List.replicate (level * 2) ' ')
 
 /- Generates a unique string identifier for a variable based on its original name and ID -/
-def var_id_ff (v : FFVar) : String :=
-  s!"{v.meta_data.orig_name}_{v.id}_L{v.meta_data.cmd_meta_data.src_info.line}"
+def varIDFF (v : FFVar) : String :=
+  s!"{v.meta_data.orig_name}_{v.id}_L{v.meta_data.src_info.row}_C{v.meta_data.src_info.col}"
 
 /- Generates a unique string identifier for a variable based on its original name and ID -/
-def var_id_bool (v : BoolVar) : String :=
-  s!"{v.meta_data.orig_name}_{v.id}_L{v.meta_data.cmd_meta_data.src_info.line}"
+def varIDBool (v : BoolVar) : String :=
+  s!"{v.meta_data.orig_name}_{v.id}_L{v.meta_data.src_info.row}_C{v.meta_data.src_info.col}"
 
 /-- Customizable variable printer (e.g., "v_0", "v_1") -/
-def print_var_ff (stream : IO.FS.Stream) (v : FFVar) : IO Unit := do
+def printVarFF (stream : IO.FS.Stream) (v : FFVar) : IO Unit := do
 --  stream.putStr s!"v_{v.id}"
-  stream.putStr s!"{var_id_ff v}"
+  stream.putStr s!"{varIDFF v}"
 
 /-- Customizable variable printer (e.g., "v_0", "v_1") -/
-def print_var_bool (stream : IO.FS.Stream) (v : BoolVar) : IO Unit := do
+def printVarBool (stream : IO.FS.Stream) (v : BoolVar) : IO Unit := do
 --  stream.putStr s!"v_{v.id}"
-  stream.putStr s!"{var_id_bool v}"
+  stream.putStr s!"{varIDBool v}"
 
 /-- Prints a term as an S-expression: (+ a b) -/
-partial def print_term {c : ZKConfig}
+def printTerm {c : ZKConfig}
   (stream : IO.FS.Stream) (t : FFTerm c) : IO Unit := do
   match t with
   | .const val =>
       stream.putStr s!"{val.val}"
   | .var v =>
-      print_var_ff stream v
+      printVarFF stream v
   | .add a b =>
       stream.putStr "(ff.add "
-      print_term stream a
+      printTerm stream a
       stream.putStr " "
-      print_term stream b
+      printTerm stream b
       stream.putStr ")"
   | .sub a b =>
       stream.putStr "(ff.sub "
-      print_term stream a
+      printTerm stream a
       stream.putStr " "
-      print_term stream b
+      printTerm stream b
       stream.putStr ")"
   | .mul a b =>
       stream.putStr "(ff.mul "
-      print_term stream a
+      printTerm stream a
       stream.putStr " "
-      print_term stream b
+      printTerm stream b
       stream.putStr ")"
 
 /- Prints the boolean formula structure -/
-partial def print_formula_body {c : ZKConfig}
+def printFormula {c : ZKConfig}
   (stream : IO.FS.Stream) (f : FFFormula c) (level : Nat) : IO Unit := do
-  let sp := get_indent level
+  let sp := getIndent level
   match f with
+  | .true  => stream.putStrLn s!"{sp}true"
+  | .false => stream.putStrLn s!"{sp}false"
   | .bool v =>
-      stream.putStr s!"{sp}{var_id_bool v}"
+      stream.putStr s!"{sp}{varIDBool v}"
   | .eqZero t =>
       stream.putStr s!"{sp}(= "
-      print_term stream t
+      printTerm stream t
       stream.putStrLn " 0)"
   | .and a b =>
       stream.putStrLn s!"{sp}(and "
-      print_formula_body stream a (level + 1)
-      print_formula_body stream b (level + 1)
+      printFormula stream a (level + 1)
+      printFormula stream b (level + 1)
       stream.putStrLn s!"{sp})"
   | .or a b =>
       stream.putStrLn s!"{sp}(or "
-      print_formula_body stream a (level + 1)
-      print_formula_body stream b (level + 1)
+      printFormula stream a (level + 1)
+      printFormula stream b (level + 1)
       stream.putStrLn s!"{sp})"
   | .ite c t e =>
       stream.putStrLn s!"{sp}(ite "
-      print_formula_body stream c (level + 1)
-      print_formula_body stream t (level + 1)
-      print_formula_body stream e (level + 1)
+      printFormula stream c (level + 1)
+      printFormula stream t (level + 1)
+      printFormula stream e (level + 1)
       stream.putStrLn s!"{sp})"
   | .imply a b =>
       stream.putStrLn s!"{sp}(=>"
-      print_formula_body stream a (level + 1)
-      print_formula_body stream b (level + 1)
+      printFormula stream a (level + 1)
+      printFormula stream b (level + 1)
       stream.putStrLn s!"{sp})"
   | .iff a b =>
       stream.putStrLn s!"{sp}(= "
-      print_formula_body stream a (level + 1)
-      print_formula_body stream b (level + 1)
+      printFormula stream a (level + 1)
+      printFormula stream b (level + 1)
       stream.putStrLn s!"{sp})"
   | .not a =>
       stream.putStrLn s!"{sp}(not "
-      print_formula_body stream a (level + 1)
+      printFormula stream a (level + 1)
       stream.putStrLn s!"{sp})"
-  | .true  => stream.putStrLn s!"{sp}true"
-  | .false => stream.putStrLn s!"{sp}false"
+  | .call name args =>
+      stream.putStr s!"{sp}({name} "
+      let argStrs := args.map (fun var =>
+        match var with
+        | .inl ffVar => varIDFF ffVar
+        | .inr boolVar => varIDBool boolVar
+      )
+      stream.putStr (String.intercalate " " argStrs)
+      stream.putStrLn ")"
 
-/- Prints the full SMT2 representation of the formula, including variable declarations
-   and the assertion. Note that it receives the list of variables to declare as input,
-   which can be obtained using `collect_vars`.
--/
-def print_smt2 {c : ZKConfig}
-    (varsFF : List FFVar)
-    (varsBool : List BoolVar)
-    (f : FFFormula c)
-    (stream : IO.FS.Stream) : IO Unit := do
-  -- Header
+
+def printMacro {c : ZKConfig}
+  (stream : IO.FS.Stream) (m : FFMacro c) : IO Unit := do
+  stream.putStr s!"(define-fun {m.name} ("
+  let paramStrs := m.params.map (fun var =>
+    match var with
+    | .inl ffVar => s!"({varIDFF ffVar} FFp)"
+    | .inr boolVar => s!"({varIDBool boolVar} Bool)"
+  )
+  stream.putStr (String.intercalate " " paramStrs)
+  stream.putStrLn ") Bool"
+  printFormula stream m.body 1
+
+def printMacros {c : ZKConfig}
+  (stream : IO.FS.Stream) (ms : List (FFMacro c)) : IO Unit := do
+  match ms with
+  | [] => return ()
+  | m :: rest =>
+      printMacro stream m
+      stream.putStrLn ""
+      stream.putStrLn ""
+      printMacros stream rest
+
+def printConstraintSystem {c : ZKConfig}
+  (stream : IO.FS.Stream) (sys : FFConstraintSystem c) : IO Unit := do
+  let (ffVars, boolVars) := collectVars sys.formula
+  printMacros stream sys.macros
+  printFormula stream sys.formula 0
   stream.putStrLn "(set-logic QF_FF)"
   stream.putStrLn ""
   -- The Finite Field sort declaration
   stream.putStrLn s!"(define-sort FFp () (_ FiniteField {c.p}))"
   -- Variable Declarations
-  for v in varsFF do
+  for v in ffVars do
     stream.putStr "(declare-const "
-    print_var_ff stream v
+    printVarFF stream v
     stream.putStrLn " FFp)"
-  for v in varsBool do
+  for v in boolVars do
     stream.putStr "(declare-const "
-    print_var_bool stream v
+    printVarBool stream v
     stream.putStrLn " Bool)"
-  -- Assertion
+  -- Macros
+  printMacros stream sys.macros.reverse -- we assume main is first
+  -- Main formula
   stream.putStrLn "(assert "
-  print_formula_body stream f 1
+  printFormula stream sys.formula 1
   stream.putStrLn ")"
   stream.flush
 
