translator/lean/llzk/Playground/Parsing.lean
@@ -3,4 +3,4 @@ import Main
 
 -- #eval main <| "-o tmp/out.txt test_progs/liveness/p3.txt".splitOn " "
 
-#eval main <| "-pp -sl test_progs/liveness/p3.txt".splitOn " "
+#eval main <| "-pp -sl test_progs/syntax/simple.txt".splitOn " "
